BlockCoordinationSystemRefinement proves; no framing yet

Splinter/BlockLayer/BlockCoordinationSystem.i.dfy
@@ -280,8 +280,7 @@ module BlockCoordinationSystem
       ))
   }
 
-  predicate CommitStart(v: Variables, v': Variables, uiop : UIOp,
-      endJournal: LSN, frozenJournal: JournalImage)
+  predicate CommitStart(v: Variables, v': Variables, uiop : UIOp, frozenJournal: JournalImage)
   {
     && uiop.NoopOp?
     && v.WF()
@@ -290,14 +289,14 @@ module BlockCoordinationSystem
     && v.inFlightImage.None?
 
     && v.ephemeral.frozenMap.Some?
-    && var startJournal := v.ephemeral.frozenMap.value.seqEnd;
+    && frozenJournal.WF()
+    && v.ephemeral.frozenMap.value.seqEnd == frozenJournal.SeqStart()
     // Frozen map can't go backwards vs persistent map, lest we end up with
     // a gap to the ephemeral journal start.
-    && v.persistentImage.mapadt.seqEnd <= startJournal
+    && v.persistentImage.mapadt.seqEnd <= frozenJournal.SeqStart()
     // And of course there should be no way for it to have passed the ephemeral map!
-    && startJournal <= v.ephemeral.mapLsn
-    && startJournal <= endJournal
-    && v.persistentImage.SeqEnd() <= endJournal
+    && frozenJournal.SeqStart() <= v.ephemeral.mapLsn
+    && v.persistentImage.SeqEnd() <= frozenJournal.SeqEnd()
 
     && MarshalledJournal.Next(v.ephemeral.journal, v'.ephemeral.journal,
         MarshalledJournal.FreezeForCommitLabel(frozenJournal))
@@ -363,7 +362,7 @@ module BlockCoordinationSystem
     | ReqSyncStep()
     | ReplySyncStep()
     | FreezeMapAdtStep()
-    | CommitStartStep(seqBoundary: LSN, frozenJournal: JournalImage)
+    | CommitStartStep(frozenJournal: JournalImage)
     | CommitCompleteStep()
     | CrashStep()
 
@@ -380,7 +379,7 @@ module BlockCoordinationSystem
       case ReqSyncStep() => ReqSync(v, v', uiop)
       case ReplySyncStep() => ReplySync(v, v', uiop)
       case FreezeMapAdtStep() => FreezeMapAdt(v, v', uiop)
-      case CommitStartStep(seqBoundary, frozenJournal) => CommitStart(v, v', uiop, seqBoundary, frozenJournal)
+      case CommitStartStep(frozenJournal) => CommitStart(v, v', uiop, frozenJournal)
       case CommitCompleteStep() => CommitComplete(v, v', uiop)
       case CrashStep() => Crash(v, v', uiop)
     }
